Add std/dlchain. Begin std/deque.std_deque.

theories/std/deque.v
@@ -1,9 +1,12 @@
 From caml5 Require Import
   prelude.
 From caml5.lang Require Import
-  notations.
+  notations
+  proofmode.
 From caml5.std Require Export
   base.
+From caml5.std Require Import
+  dlchain.
 
 Record deque `{!heapGS Σ} := {
   deque_make : val ;
@@ -59,3 +62,156 @@ Record deque `{!heapGS Σ} := {
 #[global] Arguments deque _ {_} : assert.
 #[global] Arguments Build_deque {_ _ _ _ _ _ _ _ _ _} _ _ _ _ _ _ : assert.
 #[global] Existing Instance deque_model_timeless.
+
+Section std_deque.
+  Context `{!heapGS Σ}.
+
+  Definition std_deque_make : val :=
+    λ: <>,
+      let: "t" := dlchain_singleton #() #() #() in
+      dlchain_set_prev "t" "t" ;;
+      dlchain_set_next "t" "t" ;;
+      "t".
+
+  Definition std_deque_is_empty : val :=
+    λ: "t",
+      dlchain_next "t" = "t".
+
+  Definition std_deque_push_front : val :=
+    λ: "t" "v",
+      let: "old_front" := dlchain_next "t" in
+      let: "front" := dlchain_singleton "t" "v" "old_front" in
+      dlchain_set_next "t" "front" ;;
+      dlchain_set_prev "old_front" "front".
+
+  Definition std_deque_pop_front : val :=
+    λ: "t",
+      if: std_deque_is_empty "t" then (
+        NONE
+      ) else (
+        let: "old_front" := dlchain_next "t" in
+        let: "front" := dlchain_next "old_front" in
+        dlchain_set_next "t" "front" ;;
+        dlchain_set_prev "front" "t" ;;
+        SOME (dlchain_data "old_front")
+      ).
+
+  Definition std_deque_push_back : val :=
+    λ: "t" "v",
+      let: "old_back" := dlchain_prev "t" in
+      let: "back" := dlchain_singleton "old_back" "v" "t" in
+      dlchain_set_next "old_back" "back" ;;
+      dlchain_set_prev "t" "back".
+
+  Definition std_deque_pop_back : val :=
+    λ: "t",
+      if: std_deque_is_empty "t" then (
+        NONE
+      ) else (
+        let: "old_back" := dlchain_prev "t" in
+        let: "back" := dlchain_prev "old_back" in
+        dlchain_set_next "old_back" "back" ;;
+        dlchain_set_prev "t" "back" ;;
+        SOME (dlchain_data "old_back")
+      ).
+
+  Definition std_deque_model t vs : iProp Σ :=
+    ∃ back, dlchain_model t (DfracOwn 1) back (#() :: vs) back t.
+
+  #[global] Instance std_deque_model_timeless t vs :
+    Timeless (std_deque_model t vs).
+  Proof.
+    apply _.
+  Qed.
+
+  Lemma std_deque_make_spec :
+    {{{ True }}}
+      std_deque_make #()
+    {{{ t, RET t; std_deque_model t [] }}}.
+  Proof.
+    iIntros "%Φ _ HΦ".
+    wp_rec.
+    wp_apply (dlchain_singleton_spec with "[//]"). iIntros "%sent Hsent".
+    wp_pures.
+    wp_apply (dlchain_set_prev_spec with "Hsent"); first (simpl; lia). iIntros "Hsent".
+    wp_pures.
+    wp_apply (dlchain_set_next_spec with "Hsent"). iIntros "%_ (Hsent & _)".
+    wp_pures.
+    iApply "HΦ". iExists sent. auto with iFrame.
+  Qed.
+
+  Lemma std_deque_is_empty_spec t vs :
+    {{{ std_deque_model t vs }}}
+      std_deque_is_empty t
+    {{{ RET #(bool_decide (vs = [])); std_deque_model t vs }}}.
+  Proof.
+    iIntros "%Φ (%back & Hsent) HΦ".
+    wp_rec.
+    wp_apply (dlchain_next_spec with "Hsent"). iIntros "%front (Hsent & Hfront)".
+    iDestruct (dlchain_model_unboxed with "Hsent") as %Hunboxed. wp_pures. clear Hunboxed.
+    destruct vs as [| v vs].
+    - iDestruct (dlchain_model_nil_2 with "Hfront") as %(-> & ->).
+      rewrite /= bool_decide_eq_true_2; last done.
+      iApply "HΦ". iExists back. auto with iFrame.
+    - iAssert ⌜t ≠ front⌝%I as %?.
+      { admit.
+      }
+      rewrite /= bool_decide_eq_false_2; last done.
+      iDestruct (dlchain_model_app_1 with "Hsent Hfront") as "Hsent".
+      iApply "HΦ". iExists back. auto with iFrame.
+  Admitted.
+
+  Lemma std_deque_push_front_spec t vs v :
+    {{{ std_deque_model t vs }}}
+      std_deque_push_front t v
+    {{{ RET #(); std_deque_model t (v :: vs) }}}.
+  Proof.
+  Admitted.
+
+  Lemma std_deque_pop_front_spec t vs :
+    {{{ std_deque_model t vs }}}
+      std_deque_pop_front t
+    {{{ w,
+      RET w;
+      (⌜vs = [] ∧ w = NONEV⌝ ∗ std_deque_model t []) ∨
+      (∃ v vs', ⌜vs = v :: vs' ∧ w = SOMEV v⌝ ∗ std_deque_model t vs')
+    }}}.
+  Proof.
+  Admitted.
+
+  Lemma std_deque_push_back_spec t vs v :
+    {{{ std_deque_model t vs }}}
+      std_deque_push_back t v
+    {{{ RET #(); std_deque_model t (vs ++ [v]) }}}.
+  Proof.
+  Admitted.
+
+  Lemma std_deque_pop_back_spec t vs :
+    {{{ std_deque_model t vs }}}
+      std_deque_pop_back t
+    {{{ w,
+      RET w;
+      (⌜vs = [] ∧ w = NONEV⌝ ∗ std_deque_model t []) ∨
+      (∃ vs' v, ⌜vs = vs' ++ [v] ∧ w = SOMEV v⌝ ∗ std_deque_model t vs')
+    }}}.
+  Proof.
+  Admitted.
+
+  Definition std_deque :=
+    Build_deque
+      std_deque_make_spec
+      std_deque_is_empty_spec
+      std_deque_push_front_spec
+      std_deque_pop_front_spec
+      std_deque_push_back_spec
+      std_deque_pop_back_spec.
+End std_deque.
+
+#[global] Opaque std_deque_make.
+#[global] Opaque std_deque_is_empty.
+#[global] Opaque std_deque_push_front.
+#[global] Opaque std_deque_pop_front.
+#[global] Opaque std_deque_push_back.
+#[global] Opaque std_deque_pop_back.
+
+#[global] Opaque std_deque_model.
